Correctness reduces to MLWE

code/security-estimates/Kyber_failure.py
@@ -9,16 +9,16 @@ def p2_cyclotomic_final_error_distribution(ps):
     :param ps: parameter set (ParameterSet)
     """
     chis = build_centered_binomial_law(ps.ks)           # LWE error law for the key
-    chie = build_centered_binomial_law(ps.ke)           # LWE error law for the ciphertext
+    chie = build_centered_binomial_law(ps.ke_ct)        # LWE error law for the ciphertext
+    chie_pk = build_centered_binomial_law(ps.ke)
     Rk = build_mod_switching_error_law(ps.q, ps.rqk)    # Rounding error public key
     Rc = build_mod_switching_error_law(ps.q, ps.rqc)    # rounding error first ciphertext
-    chiRs = chis # law_convolution(chis, Rk)            # LWE $ +Rounding error key
+    chiRs = law_convolution(chis, Rk)                   # LWE+Rounding error key
     chiRe = law_convolution(chie, Rc)                   # LWE + rounding error ciphertext
 
-    B1 = law_product(chie, chiRs)                       # (LWE+Rounding error) * LWE (as in a E*S product)
+    B1 = law_product(chie_pk, chiRs)                       # (LWE+Rounding error) * LWE (as in a E*S product)
     B2 = law_product(chis, chiRe)
-    # B1 => ei[i] * s[i]
-    # B2 => s[i] * (ei[i] + cu[i]) = (s[i] * ei[i]) + (s[i] * cu[i])
+
     C1 = iter_law_convolution(B1, ps.m * ps.n)
     C2 = iter_law_convolution(B2, ps.m * ps.n)
 
@@ -27,16 +27,10 @@ def p2_cyclotomic_final_error_distribution(ps):
     R2 = build_mod_switching_error_law(ps.q, ps.rq2)    # Rounding2 (in the ciphertext mask part)
     F = law_convolution(R2, chie)                       # LWE+Rounding2 error
     D = law_convolution(C, F)                           # Final error
-    DwithoutR2 = law_convolution(C, chie)               # Final error without R2
-    return (D,DwithoutR2)
+    return D
 
 
 def p2_cyclotomic_error_probability(ps):
-    (D,DwithoutR2) = p2_cyclotomic_final_error_distribution(ps)
-    e = worst_mod_switching_error(ps.q,ps.rq2)
-    print ("Worst case v error: "+ str(e))
-    proba = tail_probability(D, ps.q/4)
-    probaWithoutR2 = tail_probability(DwithoutR2, ps.q/4 - e)
-    return D, ps.n*proba, DwithoutR2, ps.n*probaWithoutR2
-
-
+    F = p2_cyclotomic_final_error_distribution(ps)
+    proba = tail_probability(F, ps.q/4)
+    return F, ps.n*proba
